\documentclass[a4paper]{article}
\usepackage[a4paper, left=5mm, right=5mm, top=5mm, bottom=5mm]{geometry}
%\geometry{paperwidth=210mm, paperheight=2000pt, left=5pt, top=5pt}
\usepackage[utf8]{inputenc}
\usepackage[english,russian]{babel}
\usepackage{indentfirst}
\usepackage{tikz}
\usepackage{cancel}
\usetikzlibrary{automata,positioning,arrows}
\usepackage{amsmath}
\usepackage{enumerate}
\usepackage{hyperref}
\usepackage{amsfonts}
\usepackage{amssymb}
\DeclareMathOperator*{\argmin}{arg\,min}
\usepackage{wasysym}
\title{}
\date{}
\author{Sergei Volodin}
\begin{document}
\maketitle
\begin{enumerate}
\item $s_t = \mbox{tanh}(W\cdot s_{t-1}+U\cdot x_t)$
\item $z_{tk}=\mbox{SoftMax}_k(V\cdot s_t)$
\item $E_t=-y_t\cdot\ln z_t$
\end{enumerate}
Then
$$\frac{\partial E_t}{\partial V}=\frac{\partial }{\partial V}(-\sum\limits_k y_{tk}\ln z_{tk})=(-\sum\limits_k y_{tk}\frac{\partial }{\partial V}\ln z_{tk})=-\sum\limits_k \frac{y_{tk}}{z_{tk}}\frac{\partial z_{tk}}{\partial V}$$


Consider
$$\frac{\partial z_{tk}}{\partial V_{ij}}=\frac{\partial}{\partial V_{ij}}\frac{e^{(V\cdot s_t)_k}}{\sum\limits_p e^{(V\cdot s_t)_p}}\boxed{=}$$

Where $(V\cdot s_t)_k=\sum\limits_s V_{ks}s_{ts}$, $\frac{\partial (V\cdot s_t)_k}{\partial V_{ij}}=\delta_{ki}s_{tj}$, $\frac{\partial e^{(V\cdot s_t)_k}}{\partial V_{ij}}=\delta_{ki}s_{tj}e^{(V\cdot s_t)_k}$, $\frac{\partial \sum\limits_p e^{(V\cdot s_t)_p}}{\partial V_{ij}}=\sum\limits_p \delta_{pi}s_{tj}e^{(V\cdot s_t)_p}=s_{tj}e^{(V\cdot s_t)_i}$


$$\boxed{=}\frac{\delta_{ki}s_{tj}e^{(V\cdot s_t)_k}\sum\limits_p e^{(V\cdot s_t)_p}-e^{(V\cdot s_t)_k}s_{tj}e^{(V\cdot s_t)_i}}{(\sum\limits_p e^{(V\cdot s_t)_p})^2}=\delta_{ki}s_{tj}z_{tk}-z_{tk}z_{ti}s_{tj}=z_{tk}s_{tj}(\delta_{ki}-z_{ti})$$

Note that $\sum\limits_k y_{tk}=1$.

Then $$\frac{\partial E_t}{\partial V_{ij}}=-\sum\limits_k \frac{y_{tk}}{z_{tk}}z_{tk}s_{tj}(\delta_{ki}-z_{ti})=-\sum\limits_k y_{tk}s_{tj}\delta_{ki}+\sum\limits_k y_{tk}s_{tj}z_{ti}=-y_{ti}s_{tj}+\sum\limits_k y_{tk} s_{tj}z_{ti}=-(y_ts_t^T)_{ij}+(z_ts_t^T)_{ij}$$

Then $\frac{\partial E_t}{\partial V}=-y_ts_t^T+z_ts_t^T=\boxed{(z_t-y_t)s_t^T}$
\end{document}